improvements to evaluation rlzr, function spaces and started reproving evaluation to be continuous.

continuity_spaces/func.v
@@ -1,6 +1,6 @@
 From mathcomp Require Import ssreflect ssrfun seq.
 From rlzrs Require Import all_rlzrs choice_dict.
-Require Import axioms all_names cs prod sub nvrsl.
+Require Import axioms all_names cs prod sub.
 
 Set Implicit Arguments.
 Unset Strict Implicit.
@@ -8,10 +8,16 @@ Unset Printing Implicit Defensive.
 
 Local Open Scope cs_scope.
 Section cs_functions.
-  Context (U: continuous_universal) (X Y: cs).
-  Local Notation F_U := (@F_M U).
-  
-  Definition associate := make_mf (fun psi (f: X -> Y) => (F_U psi) \realizes f).
+  Context (X Y: cs).
+
+  Definition function_names (B B': naming_space): naming_space.
+    exists (seq (questions B * answers B) * (questions B'))%type (seq (questions B) + answers B')%type.
+    apply/(nil, someq).
+    apply/prod_count/naming_spaces.Q_count/list_count/prod_count/naming_spaces.A_count/naming_spaces.Q_count.
+    exact/sum_count/naming_spaces.A_count/list_count/naming_spaces.Q_count.
+  Defined.
+
+  Definition associate := make_mf (fun psi (f: X -> Y) => \F_(U psi) \realizes f).
 
   Local Notation "X c-> Y" := (codom associate) (at level 2).
 
@@ -28,30 +34,66 @@ Section cs_functions.
   Qed.
 
   Canonical cs_fun: cs.
-    exists {x | x \from X c-> Y} (function_names U B_ _ B_ _) function_representation.
+    exists {x | x \from X c-> Y} (function_names B_ _ B_ _) function_representation.
     by split; [apply/fun_rep_sur | apply/fun_rep_sing].
   Defined.
 
-  Definition evaluation (fx: cs_prod cs_fun X) := (projT1 fx.1) fx.2.
+  Definition evaluation (fx: cs_prod cs_fun X) := (projT1 fx.1) fx.2.  
+
+  Local Open Scope name_scope.
+  Definition eval_rlzrM (psiphi: function_names B_(X) B_(Y) \*_ns B_(X)) :=
+    U (lprj psiphi) (rprj psiphi).
+
+  Lemma map_lstn T T' (K: seq T) (f: T -> T') q:
+    q \from L2SS K -> f q \from L2SS (map f K).
+  Proof. by elim: K => // q' K' ih /=[<- | /ih]; [left | right]. Qed.
+    
+  Lemma map_subl T T' (K K': seq T) (f: T -> T'):
+    K \is_sublist_of K' -> (map f K) \is_sublist_of (map f K').
+  Proof.
+    elim: K K' => [K' _ q | q K ih K' subl q' /=[<- | lstn]]//; first by apply/map_lstn/subl; left.
+    by apply/ih/lstn => ? ?; apply/subl; right.
+  Qed.
   
-  Definition eval_rlzr:=
-    make_mf (fun psiphi => F_U (lprj psiphi: function_names U (name_space X) (name_space Y)) (rprj psiphi)).
-  
+  Lemma eval_rlzrM_cntf: eval_rlzrM \is_continuous_functional.
+  Proof.
+    move => psiphi.
+    exists (fun nq' =>
+              map inr (gather_queries (lprj psiphi) (rprj psiphi) nq')
+                  ++ map inl (gather_queries (D (rprj psiphi)) (lprj psiphi) nq')
+           ); case => n q' psiphi'.
+    elim: n => // n.
+    rewrite /eval_rlzrM => ih /coin_cat [coin coin'].
+    rewrite /eval_rlzrM US [RHS]US ih; last first.
+    - apply/coin_cat; split; first exact/coin_subl/coin/map_subl/gq_mon.
+      exact/coin_subl/coin'/map_subl/gq_mon.
+    case: U => //.
+  Admitted.
+  Local Close Scope name_scope.
+
+  Definition eval_rlzr:= get_partial_function eval_rlzrM.
+
+  Lemma eval_rlzr_cntop: eval_rlzr \is_continuous_operator.
+  Proof. exact/gtpf_cntf_cont/eval_rlzrM_cntf. Qed.
+    
   Lemma eval_rlzr_val psiphi:
-    eval_rlzr psiphi === F_U (lprj psiphi) (rprj psiphi).
-  Proof. done. Qed.
+    PF2MF eval_rlzr psiphi === \F_(U (lprj psiphi)) (rprj psiphi).
+  Proof.
+    rewrite gtpf_spec -FMop.sing_sfrst //.    
+    by apply/FMop.mon_sing => psiphi'; have mon := @U_mon _ _ _ _ (lprj psiphi'); apply/mon.
+  Qed.
   
   Lemma eval_rlzr_crct: eval_rlzr \realizes evaluation.
   Proof.
-    rewrite rlzr_F2MF => phi [[f fhcr] x] [[_ [/=<-  [phinf phinx]]]].
+    rewrite rlzr_F2MF => phi [[f fhcr] x] [[_ [<-  [phinf phinx]]]].
     rewrite /function_representation/= in phinf.
     split => [ | Fphi RphiFphi]; last first.
-    - by apply/rlzr_val_sing; [apply/F2MF_sing | apply/phinf | apply/phinx | | ].
+    - by apply/rlzr_val_sing; [apply/F2MF_sing | | apply/phinx | | apply/eval_rlzr_val ].
     have [ | Fphi FphiFphi]:= ntrvw.rlzr_dom phinf phinx; first by apply F2MF_tot.
     by exists Fphi; apply/eval_rlzr_val.
   Qed.
 End cs_functions.
-Notation "X c-> Y" := (cs_fun F_U X Y) (at level 2): cs_scope.
+Notation "X c-> Y" := (cs_fun X Y) (at level 2): cs_scope.
 
 Section associates.
   Definition id_ass X KLq := match KLq.1: seq (queries X * replies X) with
@@ -65,7 +107,7 @@ Section associates.
     by move => phi _ <- q'; exists 2; rewrite /U/=.
   Qed.
   
-  Lemma id_ass_spec X: associate F_U X X (@id_ass X) id.
+  Lemma id_ass_spec X: associate X X (@id_ass X) id.
   Proof. exact/ntrvw.tight_rlzr/eval_F2MF/id_ass_eval/id_rlzr. Qed.
   
   Definition fst_ass X Y
@@ -81,7 +123,7 @@ Section associates.
     by move => phi _ <- q'; exists 2; rewrite /U /=.
   Qed.
   
-  Lemma fst_ass_spec X Y: associate F_U _ X (@fst_ass X Y) fst.
+  Lemma fst_ass_spec X Y: associate _ X (@fst_ass X Y) fst.
   Proof. exact/ntrvw.tight_rlzr/eval_F2MF/fst_ass_eval/fst_rlzr_spec. Qed.
   
   Definition snd_ass X Y
@@ -97,7 +139,6 @@ Section associates.
     by move => phi _ <- q'; exists 2; rewrite /U /=.
   Qed.
   
-  Lemma snd_ass_spec X Y: associate F_U _ Y (@snd_ass X Y) snd.
+  Lemma snd_ass_spec X Y: associate _ Y (@snd_ass X Y) snd.
   Proof. exact/ntrvw.tight_rlzr/eval_F2MF/snd_ass_eval/snd_rlzr_spec. Qed.
 End associates.
-
