continuity_spaces/classical_func.v
@@ -8,12 +8,10 @@ Unset Strict Implicit.
 Unset Printing Implicit Defensive.
 
 Local Open Scope cs_scope.
-Lemma ass_cont (X Y: cs) (f: X -> Y): f \from (codom (@associate F_U X Y)) -> f \is_continuous.
-Proof.
-  by move => [psi /=rlzr]; exists (F_U _ _ psi); split; first exact/FU_cont.
-Qed.
+Lemma ass_cont (X Y: cs) (f: X -> Y): f \from (codom (associate X Y)) -> f \is_continuous.
+Proof. by move => [psi /= rlzr]; exists (\F_(U psi)); split; try apply/FU_cont. Qed.
 
-Lemma cfun_spec (X Y: cs) (f: X -> Y): f \from (codom (@associate F_U X Y)) <-> f \is_continuous.
+Lemma cfun_spec (X Y: cs) (f: X -> Y): f \from (codom (associate X Y)) <-> f \is_continuous.
 Proof.
   split => [ | [F [cont rlzr]]]; first exact/ass_cont.
   have [psi val]:= exists_associate (Q_count X) (A_count X) (Q_count Y) cont.
@@ -54,88 +52,28 @@ Notation "g \o_cs f" := (cs_comp f g) (at level 29): cs_scope.
 
 Lemma cs_comp_spec (X Y Z: cs)(f: X c-> Y) (g: Y c-> Z): projT1 (g \o_cs f) =1 (projT1 g \o_f projT1 f).
 Proof. done. Qed.
- 
-Local Open Scope name_scope.
-Lemma eval_rlzr_cntop (X Y: cs):
-  (eval_rlzr F_U X Y)|_(dom (rep (cs_prod (X c-> Y) X))) \is_continuous_operator.
-Proof.
-  (*
-  rewrite !cntop_spec => psiphi [Fpsiphi [[[f x] [psinf phinx]] /eval_rlzr_val val]].
-  rewrite /= in psinf phinx; have phifd: (rprj psiphi) \from dom (F_U _ _  (lprj psiphi)) by exists Fpsiphi.
-  have [FqM [FsM prp]]:= @FM_cont_spec (queries X) (queries Y) (answers X) (answers Y).
-  have [subs [subs' [c_prp _]]]:= prp (lprj psiphi) (rprj psiphi).
-  have [qf qvl]:= subs (rprj psiphi) phifd.
-  have [sf svl]:= subs' (rprj psiphi) phifd.
-  move: subs subs' => _ _.
-  have [qfmodF [qfmodqF _]]:= c_prp qf qvl.
-  move: c_prp => _.
-  exists (fun q' => map inl (sf q') ++ map inr (qf q')) => q'.
-  exists (Fpsiphi q') => psi'phi' /coin_cat[coin coin'].
-  have : (rprj psiphi) \and (rprj psi'phi') \coincide_on (qf q').
-  - by elim: (qf q') coin' => // q K ih /= [eq /ih]; split; first rewrite /rprj /= eq.
-  have: (lprj psiphi) \and (lprj psi'phi') \coincide_on (sf q').
-  - by elim: (sf q') coin => // q K ih /= [eq /ih]; split; first rewrite /lprj /= eq.
-  move: coin coin' => _ _ coin coin'.  
-  apply det_restr => [[[f' x'] [/=psi'nf' phi'nx']]] Fpsi'phi'/eval_rlzr_val val'.
-  rewrite /= in psi'nf' phi'nx'; pose psiphi':= name_pair (lprj psiphi) (rprj psi'phi').
-  have psiphi'nfx': psiphi' \is_name_of (f, x') by trivial.
-  have [Fpsiphi' val'']: psiphi' \from dom (eval_rlzr X Y).
-  - by have []:= eval_rlzr_crct psiphi'nfx'; first exact/F2MF_dom.
-  have crt := crt_icf val (qfmodF q') _.
-  rewrite -(crt (rprj psi'phi') _ Fpsiphi' val''); last by apply/coin'.
-  have [subs [subs' [cprp _]]]:= prp (lprj psiphi) (rprj psi'phi').
-  have [ | qf' qvl']:= subs (rprj psi'phi'); first by exists Fpsiphi'.
-  move: subs subs' => _ _.
-  have [_ [_ qf'modsF]]:= cprp qf' qvl'.
-  move: cprp => _.
-  have mfeq: qf q' = qf' q'.  
-  - have [a' crt'] := qfmodqF q'.
-    suff ->: qf' q' = a' by apply/crt'; first apply/coin_ref.
-    by apply/crt'; first apply/coin'.
-  have [_ [subs' [_ vprp]]]:= prp (lprj psiphi) (rprj psi'phi').
-  have [ | sf' svl']:= subs' (rprj psi'phi'); first by exists Fpsiphi'.
-  have [sfmodF _]:= vprp sf' svl'.
-  move: vprp prp => _ _.
-  have eq: sf q' = sf' q'.
-  - have [a' crt']:= qf'modsF q'.
-    have ->: sf' q' = a' by apply/crt'; first by rewrite -mfeq; apply/coin_ref.
-    by apply/crt'; first by rewrite -mfeq; apply/coin_sym/coin'.
-  have [a' crt']:= sfmodF q'.
-  have ->: Fpsi'phi' q' = a' by apply/crt'; first by rewrite -eq; apply/coin.
-  by symmetry; apply/crt'; first by rewrite -eq; apply/coin_ref.
-Qed.*)
-Admitted.
-Local Close Scope name_scope.
 
 Lemma id_cont (X: cs): (@id X) \is_continuous.
 Proof.
-  exists (F_U _ _ (@id_ass X)).
+  exists (\F_(U (@id_ass X))).
   split; last exact/id_ass_spec.
   exact/FU_cont.
 Qed.
 
-Lemma eval_cont (X Y: cs): (@evaluation F_U X Y) \is_continuous.
-Proof.
-  exists (eval_rlzr F_U X Y)|_(dom delta).
-  split; first exact/eval_rlzr_cntop.
-  rewrite rlzr_F2MF => psiphi fx psiphinfx.
-  have [ | [Fpsiphi val] prp]:= eval_rlzr_crct psiphinfx; first exact/F2MF_dom.
-  split => [ | Fq [/=_ val']]; first by exists Fpsiphi; split; first by exists fx.
-  by have [f'x' [nm ->]]:= prp Fq val'.                         
-Qed.
+Lemma eval_cont (X Y: cs): (@evaluation X Y) \is_continuous.
+Proof. by exists (eval_rlzr X Y); split; try exact/eval_rlzr_cntop; exact/eval_rlzr_crct. Qed.
 
 Definition pt_eval (X Y: cs) (x: X) (f: X c-> Y):= evaluation (f, x).
 
 Lemma ptvl_val_cont (X Y: cs) (x: X): (@pt_eval X Y x) \is_continuous.
 Proof.
   have [phi phinx]:= get_description x.
-  exists (F_U _ _ (D phi: function_names F_U (function_names F_U _ _) _)).
-  rewrite rlzr_F2MF.
+  exists (\F_(U (D phi))).
   split => [ | psi f psinf]; try exact/FU_cont.
   have [ | [Fphi /D_spec val] prp]:= psinf phi x phinx; first exact/F2MF_dom.
   split => [ | Fphi' /D_spec val']; first by exists Fphi.
   have [fa [Fphi'nfa]]:= prp Fphi' val'.
-  by rewrite /pt_eval /evaluation =>/= ->.
+  by rewrite /pt_eval /evaluation =>/= ->; exists fa.
 Qed.
 
 Definition point_evaluation (X Y: cs) (x: X):= exist_c (@ptvl_val_cont X Y x).
